`MstoreEquivalence.lean`: remove spurious `_Val*` in LHS

EvmEquivalence/Equivalence/MstoreEquivalence.lean
@@ -14,7 +14,7 @@ namespace MstoreOpcodeEquivalence
 
 def mstoreLHS
   {GAS_CELL MEMORYUSED_CELL PC_CELL W0 W1 : SortInt}
-  {LOCALMEM_CELL _Val14 _Val15 _Val16 : SortBytes}
+  {LOCALMEM_CELL : SortBytes}
   {SCHEDULE_CELL : SortSchedule}
   {USEGAS_CELL : SortBool}
   {WS : SortWordStack}
@@ -206,14 +206,14 @@ theorem rw_mstoreLHS_mstoreRHS
   (defn_Val25 : «#memoryUsageUpdate» MEMORYUSED_CELL W0 32 = some _Val25)
   (req : _Val13 = true) :
   Rewrites
-  (@mstoreLHS GAS_CELL MEMORYUSED_CELL PC_CELL W0 W1 LOCALMEM_CELL _Val14 _Val15 _Val16 SCHEDULE_CELL USEGAS_CELL WS _DotVar0 _DotVar2 _Gen0 _Gen1 _Gen10 _Gen11 _Gen12 _Gen13 _Gen14 _Gen15 _Gen16 _Gen17 _Gen18 _Gen19 _Gen2 _Gen20 _Gen21 _Gen3 _Gen4 _Gen5 _Gen6 _Gen7 _Gen8 _Gen9 _K_CELL)
+  (@mstoreLHS GAS_CELL MEMORYUSED_CELL PC_CELL W0 W1 LOCALMEM_CELL SCHEDULE_CELL USEGAS_CELL WS _DotVar0 _DotVar2 _Gen0 _Gen1 _Gen10 _Gen11 _Gen12 _Gen13 _Gen14 _Gen15 _Gen16 _Gen17 _Gen18 _Gen19 _Gen2 _Gen20 _Gen21 _Gen3 _Gen4 _Gen5 _Gen6 _Gen7 _Gen8 _Gen9 _K_CELL)
   (@mstoreRHS _Val17 _Val24 _Val25 _Val16 SCHEDULE_CELL WS _DotVar0 _DotVar2 _Gen0 _Gen1 _Gen10 _Gen11 _Gen12 _Gen13 _Gen14 _Gen15 _Gen16 _Gen17 _Gen18 _Gen19 _Gen2 _Gen20 _Gen21 _Gen3 _Gen4 _Gen5 _Gen6 _Gen7 _Gen8 _Gen9 _K_CELL)
   := by apply (@Rewrites.MSTORE_SUMMARY_MSTORE_SUMMARY_USEGAS GAS_CELL MEMORYUSED_CELL PC_CELL W0 W1 _Val0 _Val1 _Val10 _Val17 _Val18 _Val19 _Val2 _Val20 _Val21 _Val22 _Val23 _Val24 _Val25 _Val3 _Val5 _Val6 _Val7 _Val8)
   <;> assumption
 
 theorem mstore_prestate_equiv
   {GAS_CELL MEMORYUSED_CELL PC_CELL W0 W1 : SortInt}
-  {LOCALMEM_CELL _Val14 _Val15 _Val16 : SortBytes}
+  {LOCALMEM_CELL : SortBytes}
   {SCHEDULE_CELL : SortSchedule}
   {USEGAS_CELL : SortBool}
   {WS : SortWordStack}
@@ -243,7 +243,7 @@ theorem mstore_prestate_equiv
   {_Gen9 : SortOutputCell}
   {_K_CELL : SortK}
   (symState : EVM.State) :
-  let lhs := (@mstoreLHS GAS_CELL MEMORYUSED_CELL PC_CELL W0 W1 LOCALMEM_CELL _Val14 _Val15 _Val16 SCHEDULE_CELL USEGAS_CELL WS _DotVar0 _DotVar2 _Gen0 _Gen1 _Gen10 _Gen11 _Gen12 _Gen13 _Gen14 _Gen15 _Gen16 _Gen17 _Gen18 _Gen19 _Gen2 _Gen20 _Gen21 _Gen3 _Gen4 _Gen5 _Gen6 _Gen7 _Gen8 _Gen9 _K_CELL)
+  let lhs := (@mstoreLHS GAS_CELL MEMORYUSED_CELL PC_CELL W0 W1 LOCALMEM_CELL SCHEDULE_CELL USEGAS_CELL WS _DotVar0 _DotVar2 _Gen0 _Gen1 _Gen10 _Gen11 _Gen12 _Gen13 _Gen14 _Gen15 _Gen16 _Gen17 _Gen18 _Gen19 _Gen2 _Gen20 _Gen21 _Gen3 _Gen4 _Gen5 _Gen6 _Gen7 _Gen8 _Gen9 _K_CELL)
   stateMap symState lhs =
   {symState with
     stack := (intMap W0) :: (intMap W1) :: wordStackMap WS
@@ -465,7 +465,7 @@ theorem step_mstore_equiv
   -- It seems we need this hypothesis to achieve equivalence of behavior from the EVMYul side
   -- We keep the original `W0small` for convenience
   (W0small_realpolitik : W0 < UInt32.size) :
-  EVM.step_mstore (Int.toNat GAS_CELL) gasCost (stateMap symState (@mstoreLHS GAS_CELL MEMORYUSED_CELL PC_CELL W0 W1 LOCALMEM_CELL _Val14 _Val15 _Val16 SCHEDULE_CELL USEGAS_CELL WS _DotVar0 _DotVar2 _Gen0 _Gen1 _Gen10 _Gen11 _Gen12 _Gen13 _Gen14 _Gen15 _Gen16 _Gen17 _Gen18 _Gen19 _Gen2 _Gen20 _Gen21 _Gen3 _Gen4 _Gen5 _Gen6 _Gen7 _Gen8 _Gen9 _K_CELL)) =
+  EVM.step_mstore (Int.toNat GAS_CELL) gasCost (stateMap symState (@mstoreLHS GAS_CELL MEMORYUSED_CELL PC_CELL W0 W1 LOCALMEM_CELL SCHEDULE_CELL USEGAS_CELL WS _DotVar0 _DotVar2 _Gen0 _Gen1 _Gen10 _Gen11 _Gen12 _Gen13 _Gen14 _Gen15 _Gen16 _Gen17 _Gen18 _Gen19 _Gen2 _Gen20 _Gen21 _Gen3 _Gen4 _Gen5 _Gen6 _Gen7 _Gen8 _Gen9 _K_CELL)) =
   .ok (stateMap {symState with execLength := symState.execLength + 1} (@mstoreRHS _Val17 _Val24 _Val25 _Val16 SCHEDULE_CELL WS _DotVar0 _DotVar2 _Gen0 _Gen1 _Gen10 _Gen11 _Gen12 _Gen13 _Gen14 _Gen15 _Gen16 _Gen17 _Gen18 _Gen19 _Gen2 _Gen20 _Gen21 _Gen3 _Gen4 _Gen5 _Gen6 _Gen7 _Gen8 _Gen9 _K_CELL))
   := by
   cases cg: (Int.toNat GAS_CELL)
@@ -567,7 +567,7 @@ theorem X_mstore_equiv
   -- We keep the original `W0small` for convenience
   (W0small_realpolitik : W0 < UInt32.size) :
   EVM.X (UInt256.toNat (intMap GAS_CELL)) symValidJumps
-  (stateMap symState (@mstoreLHS GAS_CELL MEMORYUSED_CELL PC_CELL W0 W1 LOCALMEM_CELL _Val14 _Val15 _Val16 SCHEDULE_CELL USEGAS_CELL WS _DotVar0 _DotVar2 _Gen0 _Gen1 _Gen10 _Gen11 _Gen12 _Gen13 _Gen14 _Gen15 _Gen16 _Gen17 _Gen18 _Gen19 _Gen2 _Gen20 _Gen21 _Gen3 _Gen4 _Gen5 _Gen6 _Gen7 _Gen8 _Gen9 _K_CELL)) =
+  (stateMap symState (@mstoreLHS GAS_CELL MEMORYUSED_CELL PC_CELL W0 W1 LOCALMEM_CELL SCHEDULE_CELL USEGAS_CELL WS _DotVar0 _DotVar2 _Gen0 _Gen1 _Gen10 _Gen11 _Gen12 _Gen13 _Gen14 _Gen15 _Gen16 _Gen17 _Gen18 _Gen19 _Gen2 _Gen20 _Gen21 _Gen3 _Gen4 _Gen5 _Gen6 _Gen7 _Gen8 _Gen9 _K_CELL)) =
   .ok (.success (stateMap {symState with execLength := symState.execLength + 2} (@mstoreRHS _Val17 _Val24 _Val25 _Val16 SCHEDULE_CELL WS _DotVar0 _DotVar2 _Gen0 _Gen1 _Gen10 _Gen11 _Gen12 _Gen13 _Gen14 _Gen15 _Gen16 _Gen17 _Gen18 _Gen19 _Gen2 _Gen20 _Gen21 _Gen3 _Gen4 _Gen5 _Gen6 _Gen7 _Gen8 ⟨.empty⟩ _K_CELL)) .empty)
   := by
   cases cg: (Int.toNat GAS_CELL)
